pcuic/theories/TemplateToPCUIC.v
@@ -1,7 +1,7 @@
 (* Distributed under the terms of the MIT license. *)
 From Coq Require Import Int63 FloatOps FloatAxioms.
 From MetaCoq.Template Require Import config utils AstUtils.
-From MetaCoq.PCUIC Require Import PCUICAst.
+From MetaCoq.PCUIC Require Import PCUICAst PCUICCases.
 
 Lemma to_Z_bounded_bool (i : Int63.int) : 
   ((0 <=? φ (i)%int63) && (φ (i)%int63 <? wB))%Z.
@@ -16,7 +16,22 @@ Definition uint63_to_model (i : Int63.int) : uint63_model :=
 Definition float64_to_model (f : PrimFloat.float) : float64_model :=
   exist _ (FloatOps.Prim2SF f) (FloatAxioms.Prim2SF_valid f).
 
-Fixpoint trans (t : Ast.term) : term :=
+Section Trans.
+  Context (Σ : PCUICAst.global_env).
+
+  Definition trans_predicate ind mdecl idecl pparams puinst pcontext preturn := 
+    let pctx := case_predicate_context_gen ind mdecl idecl pparams puinst pcontext in
+    {| pparams := pparams; 
+       puinst := puinst;
+       pcontext := pctx;
+       preturn := preturn |}.
+
+  Definition trans_branch ind mdecl cdecl pparams puinst bcontext bbody :=
+    let bctx := case_branch_context_gen ind mdecl pparams puinst bcontext cdecl in
+    {| bcontext := bctx; 
+       bbody := bbody |}.
+
+  Fixpoint trans (t : Ast.term) : term :=
   match t with
   | Ast.tRel n => tRel n
   | Ast.tVar n => tVar n
@@ -30,10 +45,25 @@ Fixpoint trans (t : Ast.term) : term :=
   | Ast.tProd na A B => tProd na (trans A) (trans B)
   | Ast.tCast c kind t => tApp (tLambda (mkBindAnn nAnon Relevant) (trans t) (tRel 0)) (trans c)
   | Ast.tLetIn na b t b' => tLetIn na (trans b) (trans t) (trans b')
-  | Ast.tCase ind p c brs =>
-    let p' := map_predicate id trans trans p in
-    let brs' := List.map (map_branch trans) brs in
-    tCase ind p' (trans c) brs'
+  | Ast.tCase ci p c brs =>
+    let p' := Ast.map_predicate id trans trans p in
+    let brs' := List.map (Ast.map_branch trans) brs in
+    match lookup_inductive Σ ci.(ci_ind) with
+    | Some (mdecl, idecl) => 
+      let tp := trans_predicate ci.(ci_ind) mdecl idecl p'.(Ast.pparams) p'.(Ast.puinst) p'.(Ast.pcontext) p'.(Ast.preturn) in
+      let tbrs := 
+        map2 (fun cdecl br => trans_branch ci.(ci_ind) mdecl cdecl 
+                  p'.(Ast.pparams) p'.(Ast.puinst) br.(Ast.bcontext) br.(Ast.bbody)) 
+                  idecl.(ind_ctors) brs' in
+      tCase ci tp (trans c) tbrs
+    | None => 
+      (** We build an ill-formed case if the term + environment are not well-formed *)
+      tCase ci {| pparams := p'.(Ast.pparams);
+                  puinst := p'.(Ast.puinst);
+                  pcontext := [];
+                  preturn := p'.(Ast.preturn) |}
+          (trans c) []
+    end
   | Ast.tProj p c => tProj p (trans c)
   | Ast.tFix mfix idx =>
     let mfix' := List.map (map_def trans trans) mfix in
@@ -45,51 +75,52 @@ Fixpoint trans (t : Ast.term) : term :=
   | Ast.tFloat n => tPrim (primFloat; primFloatModel (float64_to_model n))
   end.
 
-Definition trans_decl (d : Ast.context_decl) :=
-  let 'Ast.mkdecl na b t := d in
-  {| decl_name := na;
-     decl_body := option_map trans b;
-     decl_type := trans t |}.
+  Definition trans_decl (d : Ast.context_decl) :=
+    let 'mkdecl na b t := d in
+    {| decl_name := na;
+      decl_body := option_map trans b;
+      decl_type := trans t |}.
 
-Definition trans_local Γ := List.map trans_decl Γ.
+  Definition trans_local Γ := List.map trans_decl Γ.
 
-Definition trans_constructor_body (d : Ast.constructor_body) :=
-  {| cstr_name := d.(Ast.cstr_name); 
-     cstr_args := trans_local d.(Ast.cstr_args);
-     cstr_indices := map trans d.(Ast.cstr_indices); 
-     cstr_type := trans d.(Ast.cstr_type);
-     cstr_arity := d.(Ast.cstr_arity) |}.
+  Definition trans_constructor_body (d : Ast.constructor_body) :=
+    {| cstr_name := d.(Ast.cstr_name); 
+      cstr_args := trans_local d.(Ast.cstr_args);
+      cstr_indices := map trans d.(Ast.cstr_indices); 
+      cstr_type := trans d.(Ast.cstr_type);
+      cstr_arity := d.(Ast.cstr_arity) |}.
 
-Definition trans_one_ind_body (d : Ast.one_inductive_body) :=
-  {| ind_name := d.(Ast.ind_name);
-     ind_relevance := d.(Ast.ind_relevance);
-     ind_indices := trans_local d.(Ast.ind_indices);
-     ind_sort := d.(Ast.ind_sort);
-     ind_type := trans d.(Ast.ind_type);
-     ind_kelim := d.(Ast.ind_kelim);
-     ind_ctors := List.map trans_constructor_body d.(Ast.ind_ctors);
-     ind_projs := List.map (fun '(x, y) => (x, trans y)) d.(Ast.ind_projs) |}.
+  Definition trans_one_ind_body (d : Ast.one_inductive_body) :=
+    {| ind_name := d.(Ast.ind_name);
+      ind_relevance := d.(Ast.ind_relevance);
+      ind_indices := trans_local d.(Ast.ind_indices);
+      ind_sort := d.(Ast.ind_sort);
+      ind_type := trans d.(Ast.ind_type);
+      ind_kelim := d.(Ast.ind_kelim);
+      ind_ctors := List.map trans_constructor_body d.(Ast.ind_ctors);
+      ind_projs := List.map (fun '(x, y) => (x, trans y)) d.(Ast.ind_projs) |}.
 
-Definition trans_constant_body bd :=
-  {| cst_type := trans bd.(Ast.cst_type); cst_body := option_map trans bd.(Ast.cst_body);
-     cst_universes := bd.(Ast.cst_universes) |}.
+  Definition trans_constant_body bd :=
+    {| cst_type := trans bd.(Ast.cst_type); cst_body := option_map trans bd.(Ast.cst_body);
+      cst_universes := bd.(Ast.cst_universes) |}.
 
-Definition trans_minductive_body md :=
-  {| ind_finite := md.(Ast.ind_finite);
-     ind_npars := md.(Ast.ind_npars);
-     ind_params := trans_local md.(Ast.ind_params);
-     ind_bodies := map trans_one_ind_body md.(Ast.ind_bodies);
-     ind_universes := md.(Ast.ind_universes);
-     ind_variance := md.(Ast.ind_variance) |}.
+  Definition trans_minductive_body md :=
+    {| ind_finite := md.(Ast.ind_finite);
+      ind_npars := md.(Ast.ind_npars);
+      ind_params := trans_local md.(Ast.ind_params);
+      ind_bodies := map trans_one_ind_body md.(Ast.ind_bodies);
+      ind_universes := md.(Ast.ind_universes);
+      ind_variance := md.(Ast.ind_variance) |}.
 
-Definition trans_global_decl (d : Ast.global_decl) :=
-  match d with
-  | Ast.ConstantDecl bd => ConstantDecl (trans_constant_body bd)
-  | Ast.InductiveDecl bd => InductiveDecl (trans_minductive_body bd)
-  end.
+  Definition trans_global_decl (d : Ast.global_decl) :=
+    match d with
+    | Ast.ConstantDecl bd => ConstantDecl (trans_constant_body bd)
+    | Ast.InductiveDecl bd => InductiveDecl (trans_minductive_body bd)
+    end.
+End Trans.
 
 Definition trans_global_decls (d : Ast.global_env) :=
-  List.map (on_snd trans_global_decl) d.
+  fold_right (fun decl Σ' => on_snd (trans_global_decl Σ') decl :: Σ') [] d.
 
 Definition trans_global (Σ : Ast.global_env_ext) :=
   (trans_global_decls (fst Σ), snd Σ).
